Split lifted STLC file into two: main theory and examples.

STLC_SuccNat/Lifted_STLC_SuccNat.v
@@ -37,8 +37,6 @@ Notation "'[[' x ']]'" := x
   (at level 0, x custom pc_syntax at level 99).
 
 (* Function that evaluates a Presence Condition given a Feature Configuration *)
-(* Q: Should I do a relational definition of this function?
-      Since it might be easier to prove something *)
 Fixpoint pc_eval (cfg : FeatureConfig) (pc : PresenceCondition) : bool :=
   match pc with
   | PC_Feature f => if in_dec String.string_dec f cfg then true else false
@@ -48,220 +46,6 @@ Fixpoint pc_eval (cfg : FeatureConfig) (pc : PresenceCondition) : bool :=
   | PC_True => true
   | PC_False => false
   end.
-
-Example pc1: pc_eval ["A"; "B"] [[ (FEATURE "A") /\ (FEATURE "B") ]] = true.
-Proof. reflexivity. Qed.
-
-Example pc2: pc_eval [] [[ ~ FEATURE "C" ]] = true.
-Proof. reflexivity. Qed.
-
-Example pc3: pc_eval ["A"; "B"; "C"] [[ (FEATURE "A") /\ ~ (FEATURE "B") \/ (FEATURE "C") ]] = true.
-Proof. reflexivity. Qed.
-
-Example pc4: pc_eval ["A"] [[ TRUE /\ (FEATURE "A") ]] = true.
-Proof. reflexivity. Qed.
-
-Example pc5: pc_eval ["A"] [[ FALSE /\ (FEATURE "A") ]] = false.
-Proof. reflexivity. Qed.
-
-(*TODO: Define a plusone because it's simpler to work with*)
-Definition plusone := abs "n" Nat (succ (var "n")).
-
-Definition plustwo := abs "n" Nat (succ (succ (var "n"))).
-
-Example ty_plusone: has_type empty plusone (Arrow Nat Nat).
-Proof.
-  apply T_Abs.
-  apply T_Succ.
-  apply T_Var.
-  reflexivity.
-Qed.
-
-Example ty_plustwo: has_type empty plustwo (Arrow Nat Nat).
-Proof.
-  apply T_Abs.
-  apply T_Succ. apply T_Succ.
-  apply T_Var. reflexivity.
-Qed.
-
-Example plusone_0_is_1:
-  step_normal_form_of (STLC_SuccNat.app plusone (const 0)) (const 1).
-Proof.
-  split.
-  - eapply multi_step.
-    + apply ST_AppAbs. apply v_nat.
-    + eapply multi_step.
-      * simpl. eapply ST_SuccConst.
-      * apply multi_refl.
-  - intros [t' Contra]. inversion Contra.
-Qed.
-
-Example plustwo_3_is_5:
-  step_normal_form_of (STLC_SuccNat.app plustwo (const 3)) (const 5).
-Proof.
-  split.
-  - eapply multi_step.
-    + apply ST_AppAbs. apply v_nat.
-    + eapply multi_step.
-      * simpl. eapply ST_Succ. apply ST_SuccConst.
-      * eapply multi_step.
-        ** apply ST_SuccConst.
-        ** apply multi_refl.
-  - intros [t' Contra]. inversion Contra.
-Qed.
-
-Definition lifted_plusone := [(abs "n" Nat (succ (var "n")), [[TRUE]])].
-
-Definition lifted_plustwo := [(abs "n" Nat (succ (succ (var "n"))), [[TRUE]])].
-Check lifted_plustwo.
-
-(* It's possible to define this like a function that receives a ty and returns a lifted_ty *)
-Definition lifted_tm := list (tm * PresenceCondition).
-
-(* Example disjoint1: disjoint [[TRUE]] [[FALSE]].
-Proof.
-  intros cfg [Hpc1 Hpc2].
-  rewrite <- Hpc1 in Hpc2.
-  simpl in Hpc2.
-  inversion Hpc2.
-Qed.
-
-Example disjoint2: ~(disjoint [[FEATURE "A"]] [[FEATURE "B"]]).
-Proof.
-  unfold disjoint; intros Hd.
-  specialize Hd with ["A"; "B"].
-  apply Hd. split; simpl; reflexivity.
-Qed.
-
-Example disjoint3:
-  (disjoint
-    [[ ~(FEATURE "A") /\ (FEATURE "B") ]]
-    [[ ~(FEATURE "A") /\ ~(FEATURE "B") ]]
-  ).
-Proof.
-  unfold disjoint.
-  intros cfg [Hpc1 Hpc2].
-  simpl in *.
-  remember (if in_dec string_dec "A" cfg then true else false) as a.
-  remember (if in_dec string_dec "B" cfg then true else false) as b.
-  destruct a, b; 
-    try (inversion Hpc1);
-    inversion Hpc2.
-Qed.
- *)
-(* Fixpoint disjointness (lftd_tm : lifted_tm) : Prop :=
-  match lftd_tm with
-  | [] => True
-  | (_, pc) :: rest =>
-      (forall t' pc', In (t', pc') rest -> disjoint pc pc') /\ disjointness rest
-  end.
- *)
-Definition lifted_x :=
-  [
-   (const 1, [[FEATURE "A"]]);
-   (const 2, [[~ (FEATURE "A") /\ (FEATURE "B")]]);
-   (const 3, [[~ (FEATURE "A") /\ ~ (FEATURE "B")]])
-  ].
-(* 
-Example disjointness_lftd_x: disjointness lifted_x.
-Proof.
-  simpl. split.
-  - intros. destruct H.
-    + inversion H; subst.
-      intros cfg [Hpc1 Hpc2].
-      simpl in *.
-      rewrite Hpc1 in Hpc2.
-      simpl in Hpc2. discriminate.
-    + destruct H.
-      * inversion H.
-        intros cfg [Hpc1 Hpc2].
-        simpl in *.
-        rewrite Hpc1 in Hpc2.
-        simpl in Hpc2. discriminate.
-      * inversion H.
-  - split.
-    + intros. destruct H.
-      * inversion H. apply disjoint3.
-      * inversion H.
-    + split; auto.
-      intros. inversion H.
-Qed. *)
-
-Definition lifted_y :=
-  [
-    (const 5, [[(FEATURE "A") /\ ~ (FEATURE "B")]]);
-    (const 4, [[FEATURE "B"]]);
-    (const 3, [[~(FEATURE "A") /\ ~(FEATURE "B")]])
-  ].
-
-(* (*Definetively can make a Ltac to solve this stuff*)
-Example disjointness_lftd_y: disjointness lifted_y.
-Proof.
-  split.
-  - intros. destruct H; inversion H.
-    + intros cfg [Hpc1 Hpc2].
-      simpl in *.
-      remember (if in_dec string_dec "A" cfg then true else false) as a.
-      remember (if in_dec string_dec "B" cfg then true else false) as b.
-      rewrite Hpc2 in Hpc1.
-      destruct a; discriminate.
-    + inversion H0.
-      intros cfg [Hpc1 Hpc2].
-      simpl in *.
-      remember (if in_dec string_dec "A" cfg then true else false) as a.
-      remember (if in_dec string_dec "B" cfg then true else false) as b.
-      destruct a, b; discriminate.
-    + inversion H0.
-  - split.
-    + intros. destruct H.
-      * inversion H.
-        intros cfg [Hpc1 Hpc2].
-        simpl in *.
-        remember (if in_dec string_dec "A" cfg then true else false) as a.
-        remember (if in_dec string_dec "B" cfg then true else false) as b.
-        rewrite Hpc1 in Hpc2.
-        destruct a; discriminate.
-      * inversion H.
-    + split.
-      * intros. inversion H.
-      * apply I.
-Qed.
-
-Definition lifted_z := [ (const 19, [[TRUE]]) ].
-
-Example disjointness_lftd_z: disjointness lifted_z.
-Proof.
-  split.
-  - intros. inversion H.
-  - apply I.
-Qed. *)
-
-(* Fixpoint lift (t:tm) : lifted_tm :=
-  match t with
-  | var s => [(var s, [[TRUE]])]
-  | STLC_SuccNat.app t1 t2 =>
-    flat_map (fun '(tm1, pc1) =>
-      map (fun '(tm2, pc2) => 
-        ((STLC_SuccNat.app tm1 tm2), (PC_And pc1 pc2))) (lift t2)) (lift t1)
-  | const n => [(const n, [[TRUE]])]
-  | succ t1 =>
-    map (fun '(tm, pc) => (succ tm, pc)) (lift t1)
-  | abs s T t1 =>
-    map (fun '(tm, pc) => (abs s T tm, pc)) (lift t1)
-  end. *)
-
-(* Example lifting_plusone: lift plusone = lifted_plusone.
-Proof.
-  unfold lifted_plusone.
-  simpl. reflexivity.
-Qed.
-
-Example lifting_plustwo: lift plustwo = lifted_plustwo.
-Proof.
-  unfold lifted_plustwo.
-  simpl. reflexivity.
-Qed.
-*)
 
 (* Automatic lifting *)
 Inductive ty' : Type :=
@@ -274,12 +58,14 @@ Fixpoint lift_ty (T : ty) : ty' :=
     | Arrow T1 T2 => Arrow' (lift_ty T1) (lift_ty T2)
   end.
 
+Definition nat' := list (nat * PresenceCondition).
+
 Inductive tm' :=
   | var' : string -> tm'
   | abs' : string ->  ty' -> tm' -> tm'
   | app' : tm' -> tm' -> tm'
 
-  | const' : (list (nat * PresenceCondition)) -> tm'
+  | const' : nat' -> tm'
   | succ' : tm' -> tm'.
 
 Fixpoint lift (t:tm) : tm':=
@@ -292,104 +78,23 @@ Fixpoint lift (t:tm) : tm':=
   | succ t => (succ' (lift t))
   end.
 
-Fixpoint derive_ty (T':ty') : ty :=
-  match T' with
-  | Nat' => Nat
-  | Arrow' T1' T2' => Arrow (derive_ty T1') (derive_ty T2')
-  end.
-
-Fixpoint derive_const_list (lst : list (nat * PresenceCondition)) (cfg : FeatureConfig) : option tm :=
-  match lst with
+Fixpoint derive (n' : nat') (cfg : FeatureConfig) : option nat :=
+  match n' with
   | [] => None
-  | (t, pc) :: rest =>
-    if pc_eval cfg pc then Some (const t)
-    else derive_const_list rest cfg
+  | (n, pc) :: rest =>
+    if pc_eval cfg pc then Some n
+    else derive rest cfg
   end.
-
-Fixpoint derive (t':tm') (cfg:FeatureConfig) : option tm :=
-  match t' with
-  | var' s => Some (var s)
-  | abs' s T' t1' =>
-    match derive t1' cfg with
-    | Some t1 => Some (abs s (derive_ty T') t1)
-    | None => None
-    end
-  | app' t1' t2' =>
-    match derive t1' cfg, derive t2' cfg with
-    | Some t1, Some t2 => Some (STLC_SuccNat.app t1 t2)
-    | _, _ => None
-    end
-  | const' n' => derive_const_list n' cfg
-  | succ' t1' =>
-    match derive t1' cfg with
-    | Some t1 => Some (succ t1)
-    | None => None
-    end
-  end.
-
-Example const1': lift (const 1) = const' [(1, [[TRUE]])].
-Proof. simpl. reflexivity. Qed.
-
-Example plusone': lift plusone = abs' "n" Nat' (succ' (var' "n")).
-Proof. simpl. reflexivity. Qed.
-
-Definition x':= const' [
-   (1, [[FEATURE "A"]]);
-   (2, [[~ (FEATURE "A") /\ (FEATURE "B")]]);
-   (3, [[~ (FEATURE "A") /\ ~ (FEATURE "B")]])
-  ].
-
-Definition y' := const' [
-    (5, [[(FEATURE "A") /\ ~ (FEATURE "B")]]);
-    (4, [[FEATURE "B"]]);
-    (3, [[~(FEATURE "A") /\ ~(FEATURE "B")]])
-  ].
-
-Definition z' := const' [ (19, [[TRUE]]) ].
 
 Definition disjoint (pc1 pc2 : PresenceCondition) : Prop :=
   forall (cfg : FeatureConfig), ~(pc_eval cfg pc1 = true /\ pc_eval cfg pc2 = true).
 
-Fixpoint disjoint_lst (l : list(nat * PresenceCondition)) : Prop :=
+Fixpoint disjointness (l : nat') : Prop :=
   match l with
   | [] => True
   | (_, pc) :: rest =>
-      (forall t' pc', In (t', pc') rest -> disjoint pc pc') /\ disjoint_lst rest
+      (forall t' pc', In (t', pc') rest -> disjoint pc pc') /\ disjointness rest
   end.
-
-Fixpoint disjointness (t' : tm') : Prop :=
-  match t' with
-  | var' s => True
-  | abs' s T' t1' => disjointness t1'
-  | app' t1' t2' => disjointness t1' /\ disjointness t2'
-  | const' n' => disjoint_lst n'
-  | succ' t1' => disjointness t1'
-  end.
-
-Lemma disjointness_x': disjointness x'.
-Proof.
-  unfold disjointness.
-  simpl. split.
-  - intros t' pc' [].
-    + injection H as []. rewrite <- H.
-      unfold disjoint; intros cfg [].
-      simpl in H0, H1.
-      destruct in_dec; discriminate.
-    + destruct H.
-      * injection H as []. rewrite <- H.
-        intros cfg []. simpl in H0, H1.
-        destruct in_dec; discriminate.
-      * destruct H.
-  - split.
-    + intros t' pc' [].
-      * injection H as []. rewrite <- H.
-        intros cfg []. simpl in H0, H1.
-        destruct in_dec; destruct in_dec; discriminate.
-      * destruct H.
-    + split.
-      * intros. destruct H.
-      * apply I.
-Qed.
 
 Inductive value' : tm' -> Prop :=
   | v_abs' : forall x T' t', value' (abs' x T' t')
@@ -423,4 +128,14 @@ Inductive step': tm' -> tm' -> Prop :=
       (const' (map (fun '(n,pc) => ((S n), pc)) n')).
 
 Definition step'_normal_form_of t' t'':=
-  (multi step t' t'' /\ normal_form step t'').
+  (multi step' t' t'' /\ normal_form step' t'').
+
+(**)
+Theorem lifting_correct: forall (t:tm) (T:ty) (s:string) (cfg: FeatureConfig) (n1' n2':nat') (n1 n2:nat),
+  (derive n1' cfg) = Some n1 ->
+  (* has_type empty (STLC_SuccNat.app (abs s T t) (const n1)) Nat -> *)
+  step_normal_form_of (STLC_SuccNat.app (abs s T t) (const n1)) (const n2) ->
+  step'_normal_form_of (app' (lift (abs s T t)) (const' n1')) (const' n2') ->
+  (derive n2' cfg) = Some n2.
+Proof.
+Admitted.
