STLC_SuccNat/Examples.v
@@ -1,0 +1,251 @@
+Require Import STLC_SuccNat.
+Require Import String List Maps.
+Import ListNotations.
+Require Import Lifted_STLC_SuccNat.
+
+(* Presence Condition Evaluation Examples *)
+Example pc: pc_eval ["A"; "B"] [[ (FEATURE "A") /\ (FEATURE "B") ]] = true.
+Proof. reflexivity. Qed.
+
+Example pc2: pc_eval [] [[ ~ FEATURE "C" ]] = true.
+Proof. reflexivity. Qed.
+
+Example pc3: pc_eval ["A"; "B"; "C"] [[ (FEATURE "A") /\ ~ (FEATURE "B") \/ (FEATURE "C") ]] = true.
+Proof. reflexivity. Qed.
+
+Example pc4: pc_eval ["A"] [[ TRUE /\ (FEATURE "A") ]] = true.
+Proof. reflexivity. Qed.
+
+Example pc5: pc_eval ["A"] [[ FALSE /\ (FEATURE "A") ]] = false.
+Proof. reflexivity. Qed.
+
+(*Example functions plusone and plustwo*)
+Definition plusone := abs "n" Nat (succ (var "n")).
+
+Definition plustwo := abs "n" Nat (succ (succ (var "n"))).
+
+Example ty_plusone: has_type empty plusone (Arrow Nat Nat).
+Proof.
+  apply T_Abs.
+  apply T_Succ.
+  apply T_Var.
+  reflexivity.
+Qed.
+
+Example ty_plustwo: has_type empty plustwo (Arrow Nat Nat).
+Proof.
+  apply T_Abs.
+  apply T_Succ. apply T_Succ.
+  apply T_Var. reflexivity.
+Qed.
+
+Example plusone_0_is_1:
+  step_normal_form_of (STLC_SuccNat.app plusone (const 0)) (const 1).
+Proof.
+  split.
+  - eapply multi_step.
+    + apply ST_AppAbs. apply v_nat.
+    + eapply multi_step.
+      * simpl. eapply ST_SuccConst.
+      * apply multi_refl.
+  - intros [t' Contra]. inversion Contra.
+Qed.
+
+Example plustwo_3_is_5:
+  step_normal_form_of (STLC_SuccNat.app plustwo (const 3)) (const 5).
+Proof.
+  split.
+  - eapply multi_step.
+    + apply ST_AppAbs. apply v_nat.
+    + eapply multi_step.
+      * simpl. eapply ST_Succ. apply ST_SuccConst.
+      * eapply multi_step.
+        ** apply ST_SuccConst.
+        ** apply multi_refl.
+  - intros [t' Contra]. inversion Contra.
+Qed.
+
+(*Automatic Lifting Examples*)
+Example const1': lift (const 1) = const' [(1, [[TRUE]])].
+Proof. simpl. reflexivity. Qed.
+
+Example plusone': lift plusone = abs' "n" Nat' (succ' (var' "n")).
+Proof. simpl. reflexivity. Qed.
+
+(*Some SPLs examples*)
+Definition x':= [
+   (1, [[FEATURE "A"]]);
+   (2, [[~ (FEATURE "A") /\ (FEATURE "B")]]);
+   (3, [[~ (FEATURE "A") /\ ~ (FEATURE "B")]])
+  ].
+
+Definition y' := [
+    (5, [[(FEATURE "A") /\ ~ (FEATURE "B")]]);
+    (4, [[FEATURE "B"]]);
+    (3, [[~(FEATURE "A") /\ ~(FEATURE "B")]])
+  ].
+
+Definition z' := [ (19, [[TRUE]]) ].
+
+(*Disjointness Invariant Exapmles*)
+Lemma disjointness_x': disjointness x'.
+Proof.
+  unfold disjointness.
+  simpl. split.
+  - intros t' pc' [].
+    + injection H as []. rewrite <- H.
+      unfold disjoint; intros cfg [].
+      simpl in H0, H1.
+      destruct in_dec; discriminate.
+    + destruct H.
+      * injection H as []. rewrite <- H.
+        intros cfg []. simpl in H0, H1.
+        destruct in_dec; discriminate.
+      * destruct H.
+  - split.
+    + intros t' pc' [].
+      * injection H as []. rewrite <- H.
+        intros cfg []. simpl in H0, H1.
+        destruct in_dec; destruct in_dec; discriminate.
+      * destruct H.
+    + split.
+      * intros. destruct H.
+      * apply I.
+Qed.
+
+Ltac solve_by_inverts n :=
+	match goal with | H : ?T  |-  _  =>
+	match type of T with Prop =>
+		solve [ inversion H;
+		match n with S (S (?n')) =>
+			subst; solve_by_inverts (S n') end ]
+	end end.
+
+(* plusone(x'|p) = (plusone'(x'))|p *)
+Example comm_plusone_x': forall (cfg:FeatureConfig) (x n:nat) (n':nat'),
+  (derive x' cfg ) = Some x ->
+  step_normal_form_of (STLC_SuccNat.app plusone (const x)) (const n) ->
+  step'_normal_form_of (app' (lift plusone) (const' x')) (const' n') ->
+  (derive n' cfg) = Some n.
+Proof.
+  unfold step_normal_form_of, step'_normal_form_of.
+  intros cfg x n n' Hd [Hmstep Hnf] [Hmstep' Hnf'].
+
+  (*Trying to simplify Hmstep*)
+  inversion Hmstep; subst.
+  inversion H; subst;
+    try (solve_by_inverts 1).
+  simpl in H0. inversion H0; subst.
+  inversion H1; subst;
+    try (solve_by_inverts 1).
+  inversion H2; subst;
+    try (solve_by_inverts 1).
+  clear Hmstep H0 H H6 H2 H1.
+
+  (*Trying to simplify Hmstep'*)
+  inversion Hmstep'; subst.
+  inversion H; subst;
+    try (solve_by_inverts 1);
+    clear Hmstep' H.
+  inversion H0; subst.
+  inversion H; subst;
+    try (solve_by_inverts 1);
+    clear H0 H.
+  simpl in H1.
+  inversion H1; subst;
+    try (solve_by_inverts 1).
+
+  (* Case analisys on the feature configuration *)
+  simpl; simpl in Hd.
+  destruct in_dec.
+  - injection Hd as Hd;
+    subst; reflexivity.
+  - destruct in_dec;
+    injection Hd as Hd;
+    subst; reflexivity.
+Qed.
+
+(* plusone(y'|p) = (plusone'(y'))|p *)
+Example comm_plusone_y: forall (cfg:FeatureConfig) (y n: nat) (n':nat'),
+  (derive y' cfg) = Some y ->
+  step_normal_form_of (STLC_SuccNat.app plusone (const y)) (const n) ->
+  step'_normal_form_of (app' (lift plusone) (const' y')) (const' n') ->
+  (derive n' cfg) = Some n.
+Proof.
+  unfold step_normal_form_of, step'_normal_form_of.
+  intros cfg y n n' Hd [Hmstep _] [Hmstep' _].
+
+  (*Simplifying Hmstep to find value of n*)
+  inversion Hmstep; subst.
+  inversion H; subst;
+    try solve_by_inverts 1;
+    clear H Hmstep.
+  inversion H0; subst.
+  inversion H; subst;
+    try solve_by_inverts 1;
+    clear H H0.
+  inversion H1; subst;
+    try solve_by_inverts 1.
+  clear H1 H6.
+
+  (*Simplifying Hmstep' to find value of n'*)
+  inversion Hmstep'; subst.
+  inversion H; subst;
+    try solve_by_inverts 1;
+    clear H Hmstep'.
+  inversion H0; subst.
+  inversion H; subst;
+    try solve_by_inverts 2;
+    clear H H0.
+  simpl in H1.
+  inversion H1; subst;
+    try solve_by_inverts 1.
+
+  (* Case analisys on the feature configuration *)
+  simpl; simpl in Hd.
+  destruct in_dec; (*destruct in_dec as many times as there are features*)
+  destruct in_dec;
+    injection Hd as Hd;
+    subst; reflexivity.
+Qed.
+
+(* plusone(z'|p) = (plusone'(z'))|p *)
+Example comm_plusone_z: forall (cfg:FeatureConfig) (z n: nat) (n':nat'),
+  (derive z' cfg) = Some z ->
+  step_normal_form_of (STLC_SuccNat.app plusone (const z)) (const n) ->
+  step'_normal_form_of (app' (lift plusone) (const' z')) (const' n') ->
+  (derive n' cfg) = Some n.
+Proof.
+  unfold step_normal_form_of, step'_normal_form_of.
+  intros cfg z n n' Hd [Hmstep _] [Hmstep' _].
+  simpl in Hd; injection Hd as Hz.
+
+  (*Simplifying Hmstep to find value of n*)
+  inversion Hmstep; subst.
+  inversion H; subst;
+    try solve_by_inverts 1;
+    clear H Hmstep.
+  inversion H0; subst.
+  inversion H; subst;
+    try solve_by_inverts 1;
+    clear H H0.
+  inversion H1; subst;
+    try solve_by_inverts 1.
+  clear H1 H6.
+
+  (*Simplifying Hmstep' to find value of n'*)
+  inversion Hmstep'; subst.
+  inversion H; subst;
+    try solve_by_inverts 1;
+    clear H Hmstep'.
+  inversion H0; subst.
+  inversion H; subst;
+    try solve_by_inverts 2;
+    clear H H0.
+  simpl in H1.
+  inversion H1; subst;
+    try solve_by_inverts 1.
+
+  simpl. reflexivity.
+Qed.
+
